coq-minuska/theories/minusl_syntax.v
@@ -6,10 +6,10 @@ From Minuska Require Import
     basic_properties
 .
 
-Variant MinusL_Decl {Σ : StaticModel} (Act : Set) :=
+Variant MinusL_Decl {Σ : StaticModel} (Label : Set) :=
 | mld_rewrite
     (lc : TermOver BuiltinOrVar) (ld : TermOver BuiltinOrVar)
-    (a : Act)
+    (a : Label)
     (rc : TermOver Expression2) (rd : TermOver Expression2)
     (scs : SideCondition)
 | mld_context
@@ -21,10 +21,10 @@ Variant MinusL_Decl {Σ : StaticModel} (Act : Set) :=
 #[export]
 Instance MinusL_Decl_eqDec
     {Σ : StaticModel}
-    (Act : Set)
-    {_eA : EqDecision Act}
+    (Label : Set)
+    {_eA : EqDecision Label}
     :
-    EqDecision (MinusL_Decl Act)
+    EqDecision (MinusL_Decl Label)
 .
 Proof.
     ltac1:(solve_decision).
@@ -32,9 +32,9 @@ Defined.
 
 Definition actions_of_decl
     {Σ : StaticModel}
-    (Act : Set)
-    (d : MinusL_Decl Act)
-    : list Act
+    (Label : Set)
+    (d : MinusL_Decl Label)
+    : list Label
 :=
 match d with
 | mld_rewrite _ _ _ a _ _ _ => [a]
@@ -44,77 +44,77 @@ end.
 
 Record MinusL_LangDef
     {Σ : StaticModel}
-    (Act : Set)
+    (Label : Set)
     : Type
  := mkMinusL_LangDef {
     mlld_isValue_c : SideCondition ;
     mlld_isNonValue_c : SideCondition ;
     mlld_isValue_var : variable ;
-    mlld_decls : list (MinusL_Decl Act) ;
+    mlld_decls : list (MinusL_Decl Label) ;
 }.
 
 Definition MinusL_LangDef_wf
     {Σ : StaticModel}
-    (Act : Set)
-    (D : MinusL_LangDef Act)
+    (Label : Set)
+    (D : MinusL_LangDef Label)
     : Prop
 :=
-    vars_of (mlld_isValue_c Act D) = {[ mlld_isValue_var Act D ]}
+    vars_of (mlld_isValue_c Label D) = {[ mlld_isValue_var Label D ]}
     /\
-    vars_of (mlld_isNonValue_c Act D) = {[ mlld_isValue_var Act D ]}
+    vars_of (mlld_isNonValue_c Label D) = {[ mlld_isValue_var Label D ]}
     /\ (
         ∀ c h scs,
-        (mld_context Act c h scs) ∈ (mlld_decls Act D) ->
-        h <> (mlld_isValue_var Act D)
+        (mld_context Label c h scs) ∈ (mlld_decls Label D) ->
+        h <> (mlld_isValue_var Label D)
         /\ (length (filter (eq h) (vars_of_to_l2r c)) = 1)
         /\ (h ∉ vars_of scs)
     )
 .
 (*
     ∀ c h Hh scs Hhscs,
-        (mld_context Act c h Hh scs Hhscs) ∈ (mlld_decls Act D) ->
-        h ∉ vars_of (mlld_isValue_scs Act D)
+        (mld_context Label c h Hh scs Hhscs) ∈ (mlld_decls Label D) ->
+        h ∉ vars_of (mlld_isValue_scs Label D)
 .
 *)
 Definition MinusL_isValue
     {Σ : StaticModel}
-    (Act : Set)
-    (D : MinusL_LangDef Act)
+    (Label : Set)
+    (D : MinusL_LangDef Label)
     :
     Expression2 -> SideCondition
 :=
-    let x := (mlld_isValue_var Act D) in
-    let c := mlld_isValue_c Act D in
+    let x := (mlld_isValue_var Label D) in
+    let c := mlld_isValue_c Label D in
     fun e => SideCondition_subst c x e
 .
 
 Definition MinusL_isNonValue
     {Σ : StaticModel}
-    (Act : Set)
-    (D : MinusL_LangDef Act)
+    (Label : Set)
+    (D : MinusL_LangDef Label)
     :
     Expression2 -> SideCondition
 :=
-    let x := (mlld_isValue_var Act D) in
-    let c := mlld_isNonValue_c Act D in
+    let x := (mlld_isValue_var Label D) in
+    let c := mlld_isNonValue_c Label D in
     fun e => SideCondition_subst c x e
 .
 
 Definition actions_of_ldef
     {Σ : StaticModel}
-    (Act : Set)
-    (D : MinusL_LangDef Act)
-    : list Act
+    (Label : Set)
+    (D : MinusL_LangDef Label)
+    : list Label
 :=
-    concat (map (actions_of_decl Act) (mlld_decls Act D))
+    concat (map (actions_of_decl Label) (mlld_decls Label D))
 .
 
 
 #[export]
 Instance VarsOf_MinusL_Decl
     {Σ : StaticModel}
-    (Act : Set)
-    : VarsOf (MinusL_Decl Act) variable
+    (Label : Set)
+    : VarsOf (MinusL_Decl Label) variable
 := {|
     vars_of := fun D => match D with
     | mld_rewrite _ lc ld _ rc rd scs => (vars_of lc) ∪ vars_of ld ∪
@@ -126,9 +126,9 @@ Instance VarsOf_MinusL_Decl
 #[export]
 Instance VarsOf_MinusL_LangDef
     {Σ : StaticModel}
-    (Act : Set)
-    : VarsOf (MinusL_LangDef Act) variable
+    (Label : Set)
+    : VarsOf (MinusL_LangDef Label) variable
 := {|
-    vars_of := fun D => union_list (vars_of <$> (mlld_decls Act D)) ; 
+    vars_of := fun D => union_list (vars_of <$> (mlld_decls Label D)) ; 
 |}.
 
